# Composing with inverses

We can also compose a function with its inverse to get composite functions
$`ff^{-1}` and $`f^{-1}f.`

We can try to find the formula for $`f^{-1}(x)` and perform composition, but
turns out we can get the result in a simpler manner by consideration the meaning
of this composition.

$`f^{-1}` is the function that reverses $`f,` so $`f^{-1}f`
will take a number, apply $`f` to it and then try to reverse the process. We
then end up with the original number. A similar argument can be made for
$`ff^{-1},`
leading us to the following results.

## Formulas

- {=$`ff^{-1}(x) = x`=}
- {=$`f^{-1}f(x) = x`=}

## Differences between the two functions

So is $`ff^{-1}(x)` and $`f^{-1}f(x)` the exact same function? Turns out that is
not true because of domain considerations. Recall that $`{D_{fg} = D_g}` so we
have

- {=$`D_{f^{-1}f} = D_f`=}
- {=$`D_{ff^{-1}} = D_{f^{-1}}`=}

```=comment
Add a picture for these graphs
```
